SestoftNU

Launchbury/SestoftNU.thy
@@ -1,41 +1,43 @@
-theory Sestoft 
+theory SestoftNU
 imports SestoftConf
 begin
 
-inductive step :: "conf \<Rightarrow> conf \<Rightarrow> bool" (infix "\<Rightarrow>" 50) where
-  app\<^sub>1:  "(\<Gamma>, App e x, S) \<Rightarrow> (\<Gamma>, e , Arg x # S)"
-| app\<^sub>2:  "(\<Gamma>, Lam [y]. e, Arg x # S) \<Rightarrow> (\<Gamma>, e[y ::= x] , S)"
-| var\<^sub>1:  "map_of \<Gamma> x = Some e \<Longrightarrow> (\<Gamma>, Var x, S) \<Rightarrow> (delete x \<Gamma>, e , Upd x # S)"
-| var\<^sub>2:  "x \<notin> domA \<Gamma> \<Longrightarrow> isLam e \<Longrightarrow> (\<Gamma>, e, Upd x # S) \<Rightarrow> ((x,e)# \<Gamma>, e , S)"
-| let\<^sub>1:  "atom ` domA \<Delta> \<sharp>* \<Gamma> \<Longrightarrow> atom ` domA \<Delta> \<sharp>* S \<Longrightarrow> (\<Gamma>, Let \<Delta> e, S) \<Rightarrow> (\<Delta>@\<Gamma>, e , S)"
+inductive step :: "conf \<Rightarrow> conf \<Rightarrow> bool" (infix "\<Rightarrow>¹" 50) where
+  app\<^sub>1:  "(\<Gamma>, App e x, S) \<Rightarrow>¹ (\<Gamma>, e , Arg x # S)"
+| app\<^sub>2:  "(\<Gamma>, Lam [y]. e, Arg x # S) \<Rightarrow>¹ (\<Gamma>, e[y ::= x] , S)"
+| var\<^sub>1:  "map_of \<Gamma> x = Some e \<Longrightarrow> (\<Gamma>, Var x, S) \<Rightarrow>¹ (delete x \<Gamma>, e , Upd x # S)"
+| var\<^sub>2:  "x \<notin> domA \<Gamma> \<Longrightarrow> isLam e \<Longrightarrow> (\<Gamma>, e, Upd x # S) \<Rightarrow>¹ ((x,e)# \<Gamma>, e , S)"
+| var\<^sub>3:  "map_of \<Gamma> x = Some e \<Longrightarrow> (\<Gamma>, Var1 x, S) \<Rightarrow>¹ (delete x \<Gamma>, e , S)"
+| let\<^sub>1:  "atom ` domA \<Delta> \<sharp>* \<Gamma> \<Longrightarrow> atom ` domA \<Delta> \<sharp>* S \<Longrightarrow> (\<Gamma>, Let \<Delta> e, S) \<Rightarrow>¹ (\<Delta>@\<Gamma>, e , S)"
 
-abbreviation steps (infix "\<Rightarrow>\<^sup>*" 50) where "steps \<equiv> step\<^sup>*\<^sup>*"
+abbreviation steps (infix "\<Rightarrow>¹\<^sup>*" 50) where "steps \<equiv> step\<^sup>*\<^sup>*"
 
 lemma SmartLet_stepI:
-   "atom ` domA \<Delta> \<sharp>* \<Gamma> \<Longrightarrow> atom ` domA \<Delta> \<sharp>* S \<Longrightarrow> (\<Gamma>, SmartLet \<Delta> e, S) \<Rightarrow>\<^sup>*  (\<Delta>@\<Gamma>, e , S)"
+   "atom ` domA \<Delta> \<sharp>* \<Gamma> \<Longrightarrow> atom ` domA \<Delta> \<sharp>* S \<Longrightarrow> (\<Gamma>, SmartLet \<Delta> e, S) \<Rightarrow>¹\<^sup>*  (\<Delta>@\<Gamma>, e , S)"
 unfolding SmartLet_def by (auto intro: let\<^sub>1)
 
-lemma lambda_var: "map_of \<Gamma> x = Some e \<Longrightarrow> isLam e  \<Longrightarrow> (\<Gamma>, Var x, S) \<Rightarrow>\<^sup>* ((x,e) # delete x \<Gamma>, e , S)"
+lemma lambda_var: "map_of \<Gamma> x = Some e \<Longrightarrow> isLam e  \<Longrightarrow> (\<Gamma>, Var x, S) \<Rightarrow>¹\<^sup>* ((x,e) # delete x \<Gamma>, e , S)"
   by (rule rtranclp_trans[OF r_into_rtranclp r_into_rtranclp])
      (auto intro: var\<^sub>1 var\<^sub>2)
 
 text {* An induction rule that skips the annoying case of a lambda taken off the heap *}
 
 lemma step_induction[consumes 2, case_names app\<^sub>1 app\<^sub>2 thunk lamvar var\<^sub>2 let\<^sub>1 refl trans]:
-  assumes "c \<Rightarrow>\<^sup>* c'"
+  assumes "c \<Rightarrow>¹\<^sup>* c'"
   assumes "\<not> boring_step c'"
   assumes app\<^sub>1:  "\<And> \<Gamma> e x S . P (\<Gamma>, App e x, S)  (\<Gamma>, e , Arg x # S)"
   assumes app\<^sub>2:  "\<And> \<Gamma> y e x S . P (\<Gamma>, Lam [y]. e, Arg x # S) (\<Gamma>, e[y ::= x] , S)"
   assumes thunk:  "\<And> \<Gamma> x e S . map_of \<Gamma> x = Some e \<Longrightarrow> \<not> isLam e \<Longrightarrow> P (\<Gamma>, Var x, S) (delete x \<Gamma>, e , Upd x # S)"
   assumes lamvar:  "\<And> \<Gamma> x e S . map_of \<Gamma> x = Some e \<Longrightarrow> isLam e \<Longrightarrow> P (\<Gamma>, Var x, S) ((x,e) # delete x \<Gamma>, e , S)"
   assumes var\<^sub>2:  "\<And> \<Gamma> x e S . x \<notin> domA \<Gamma> \<Longrightarrow> isLam e \<Longrightarrow> P (\<Gamma>, e, Upd x # S) ((x,e)# \<Gamma>, e , S)"
+  assumes var1:  "\<And> \<Gamma> x e S .  map_of \<Gamma> x = Some e  \<Longrightarrow> P (\<Gamma>, Var1 x, S) (delete x \<Gamma>, e, S)"
   assumes let\<^sub>1:  "\<And> \<Delta> \<Gamma> e S . atom ` domA \<Delta> \<sharp>* \<Gamma> \<Longrightarrow> atom ` domA \<Delta> \<sharp>* S \<Longrightarrow> P (\<Gamma>, Let \<Delta> e, S) (\<Delta>@\<Gamma>, e, S)"
   assumes refl: "\<And> c. P c c"
-  assumes trans[trans]: "\<And> c c' c''. c \<Rightarrow>\<^sup>* c' \<Longrightarrow> c' \<Rightarrow>\<^sup>* c'' \<Longrightarrow> P c c' \<Longrightarrow> P c' c'' \<Longrightarrow> P c c''"
+  assumes trans[trans]: "\<And> c c' c''. c \<Rightarrow>¹\<^sup>* c' \<Longrightarrow> c' \<Rightarrow>¹\<^sup>* c'' \<Longrightarrow> P c c' \<Longrightarrow> P c' c'' \<Longrightarrow> P c c''"
   shows "P c c'"
 proof-
   from assms(1)
-  have "P c c' \<or> (boring_step c' \<and> (\<forall> c''. c' \<Rightarrow> c'' \<longrightarrow> P c c''))"
+  have "P c c' \<or> (boring_step c' \<and> (\<forall> c''. c' \<Rightarrow>¹ c'' \<longrightarrow> P c c''))"
   proof(induction)
   case base
     have "P c c" by (rule refl)
@@ -47,9 +49,9 @@ proof-
     proof
       assume "P c y"
 
-      note t = trans[OF `c \<Rightarrow>\<^sup>* y` r_into_rtranclp[where r = step, OF `y \<Rightarrow> z`]]
+      note t = trans[OF `c \<Rightarrow>¹\<^sup>* y` r_into_rtranclp[where r = step, OF `y \<Rightarrow>¹ z`]]
       
-      from `y \<Rightarrow> z`
+      from `y \<Rightarrow>¹ z`
       show ?thesis
       proof (cases)
         case app\<^sub>1 hence "P y z" using assms(3) by metis
@@ -65,12 +67,12 @@ proof-
           with `P c y` show ?thesis by (metis t)
         next
           case True
-          have *: "y \<Rightarrow>\<^sup>* ((x,e) # delete x \<Gamma>, e , S)" using var\<^sub>1 True lambda_var by metis
+          have *: "y \<Rightarrow>¹\<^sup>* ((x,e) # delete x \<Gamma>, e , S)" using var\<^sub>1 True lambda_var by metis
 
           have "boring_step (delete x \<Gamma>, e, Upd x # S)" using True ..
           moreover
           have "P y ((x,e) # delete x \<Gamma>, e , S)" using var\<^sub>1 True assms(6) by metis
-          with `P c y` have "P c ((x,e) # delete x \<Gamma>, e , S)" by (rule trans[OF `c \<Rightarrow>\<^sup>* y` *])
+          with `P c y` have "P c ((x,e) # delete x \<Gamma>, e , S)" by (rule trans[OF `c \<Rightarrow>¹\<^sup>* y` *])
           ultimately
           show ?thesis using var\<^sub>1(2,3) True by (auto elim!: step.cases)
         qed
@@ -78,12 +80,15 @@ proof-
         case var\<^sub>2 hence "P y z" using assms(7) by metis
         with `P c y` show ?thesis by (metis t)
       next
-        case let\<^sub>1 hence "P y z" using assms(8) by metis
+        case var\<^sub>3 hence "P y z" using assms(8) by metis
+        with `P c y` show ?thesis by (metis t)
+      next
+        case let\<^sub>1 hence "P y z" using assms(9) by metis
         with `P c y` show ?thesis by (metis t)
       qed
     next
-      assume "boring_step y \<and> (\<forall>c''. y \<Rightarrow> c'' \<longrightarrow> P c c'')"
-      with `y \<Rightarrow> z`
+      assume "boring_step y \<and> (\<forall>c''. y \<Rightarrow>¹ c'' \<longrightarrow> P c c'')"
+      with `y \<Rightarrow>¹ z`
       have "P c z" by blast
       thus ?thesis..
     qed
@@ -91,5 +96,6 @@ proof-
   with assms(2)
   show ?thesis by auto
 qed
+
 
 end
