Launchbury/SestoftConf.thy
@@ -1,0 +1,62 @@
+theory SestoftConf
+imports Terms Substitution
+begin
+
+datatype stack_elem = Arg var | Upd var | Dummy var
+
+instantiation stack_elem :: pt
+begin
+definition  "\<pi> \<bullet> x = (case x of (Arg v) \<Rightarrow> Arg (\<pi> \<bullet> v) | (Upd v) \<Rightarrow> Upd (\<pi> \<bullet> v) | (Dummy v) \<Rightarrow> Dummy (\<pi> \<bullet> v))"
+instance
+  by default (auto simp add: permute_stack_elem_def split:stack_elem.split)
+end
+
+lemma Arg_eqvt[eqvt]: "\<pi> \<bullet> (Arg v) = Arg (\<pi> \<bullet> v)"
+  and Upd_eqvt[eqvt]: "\<pi> \<bullet> (Upd v) = Upd (\<pi> \<bullet> v)"
+  and Dummy_eqvt[eqvt]: "\<pi> \<bullet> (Dummy v) = Dummy (\<pi> \<bullet> v)"
+  by (auto simp add: permute_stack_elem_def split:stack_elem.split)
+
+lemma supp_Arg[simp]: "supp (Arg v) = supp v"  unfolding supp_def by auto
+lemma supp_Upd[simp]: "supp (Upd v) = supp v"  unfolding supp_def by auto
+lemma supp_Dummy[simp]: "supp (Dummy v) = supp v"  unfolding supp_def by auto
+lemma fresh_Arg[simp]: "a \<sharp> Arg v = a \<sharp> v" unfolding fresh_def by auto
+lemma fresh_Upd[simp]: "a \<sharp> Upd v = a \<sharp> v" unfolding fresh_def by auto
+lemma fresh_Dummy[simp]: "a \<sharp> Dummy v = a \<sharp> v" unfolding fresh_def by auto
+lemma fv_Arg[simp]: "fv (Arg v) = fv v"  unfolding fv_def by auto
+lemma fv_Upd[simp]: "fv (Upd v) = fv v"  unfolding fv_def by auto
+
+instance stack_elem :: fs  by (default, case_tac x) (auto simp add: finite_supp)
+
+type_synonym stack = "stack_elem list"
+
+
+fun ap :: "stack \<Rightarrow> var set" where
+  "ap [] = {}"
+| "ap (Arg x # S) = insert x (ap S)"
+| "ap (Upd x # S) = ap S"
+| "ap (Dummy x # S) = ap S"
+fun upds :: "stack \<Rightarrow> var set" where
+  "upds [] = {}"
+| "upds (Upd x # S) = insert x (upds S)"
+| "upds (Arg x # S) = upds S"
+| "upds (Dummy x # S) = upds S"
+fun flattn :: "stack \<Rightarrow> var list" where
+  "flattn [] = []"
+| "flattn (Upd x # S) = x # flattn S"
+| "flattn (Arg x # S) = x # flattn S"
+| "flattn (Dummy x # S) = x # flattn S"
+
+lemma ups_fv_subset: "upds S \<subseteq> fv S"
+  by (induction S rule: upds.induct) auto
+
+lemma fresh_flattn[simp]: "a \<sharp> flattn S \<longleftrightarrow> a \<sharp> S"
+  by (induction S rule:flattn.induct) (auto simp add: fresh_Nil fresh_Cons)
+lemma fresh_star_flattn[simp]: "a \<sharp>* flattn S \<longleftrightarrow> a \<sharp>* S"
+  by (auto simp add: fresh_star_def)
+
+type_synonym conf = "(heap \<times> exp \<times> stack)"
+
+inductive boring_step where
+  "isLam e \<Longrightarrow> boring_step (\<Gamma>, e, Upd x # S)"
+
+end
